Done

Exercises/SolutionWeek3.lean
@@ -1,6 +1,21 @@
+/-
+Proving theorems in Lean: Lean and Mathlib for bigger projects.
+Yuval Filmus, Shachar Itzhaky, ∧ Jonathan Reicher, 2025
+-/
+
 import Mathlib.Tactic
 
 
+/-
+In this file, we will learn using programming concepts such as types and namespaces,
+to help us in defining mathematics, and to make proofs easy to construct.
+
+You will learn about: `namespace`, `inductive`, `structure`, `Type`, `Prop`
+`Subtype`, `class`, `Finset`, .
+-/
+
+
+-- First exercise:
 -- Let's prove that barbers do not exist.
 -- The Barber Paradox is a just a logical statement which one might find
 -- suprising.
@@ -10,15 +25,51 @@ structure Person where
   name : String
 
 
-structure IsBarber (b : Person) where
-  shaves : Person → Person → Prop -- A relation over two elements
-  proof : ∀ p : Person, shaves b p ↔ ¬ shaves p p
+structure Town where
+  people : Finset Person
+  shaves : (p₁ : Person) → (p₂ : Person) → p₁ ∈ people → p₂ ∈ people → Prop
 
 
-theorem paradox (b : Person) : IsBarber b → False := by
-  intro h
+/--
+This abbreviation let's us use `Resident t` as a shorthand for `{ p // p ∈ t.people }`.
+`{ p // p ∈ t.people }` is a `Subtype Person`. It is a new type, containing all `Person` that
+are members of the town.
+-/
+abbrev Resident (t : Town) : Type := { p // p ∈ t.people }
+
+
+/--
+This abbreviation is under the `Resident` namespace. That means that you can use `a.shaves b`
+as a short for `t.shaves a b` when `a : Resident t`.
+-/
+abbrev Resident.shaves {t : Town} (a b : Resident t) :=
+  t.shaves a b a.property b.property
+/-
+Could have also written it as:
+namespace Resident
+
+abbrev shaves {t : Town} (a b : Resident t) :=
+  t.shaves a b a.property b.property
+
+end Resident
+-/
+
+
+/-- And this is a function to construct a `Resident t` -/
+def Resident.mk (t : Town) (p : Person) (h : p ∈ t.people) : Resident t := ⟨p, h⟩
+
+
+-- This structure is different: the `: Prop` below makes this type a proposition. In practice,
+-- propositions and regular types are almost the same. We will see the difference later.
+structure IsBarber {t : Town} (b : Resident t) : Prop where
+  proof : ∀ p, b.shaves p ↔ ¬ p.shaves p
+
+
+theorem paradox : ¬ ∃ t, ∃ b : Resident t, IsBarber b := by
+  by_contra! h
+  obtain ⟨t, b, h⟩ := h
   obtain hB := h.proof b
-  by_cases h.shaves b b
+  by_cases b.shaves b
   case pos hShaves =>
     have hNotShaves := hB.mp hShaves
     contradiction
@@ -31,26 +82,186 @@ theorem paradox (b : Person) : IsBarber b → False := by
 -- Of course, that's just because of our flawed definition
 
 
-structure IsBarber' (b : Person) where
-  shaves : Person → Person → Prop -- A relation over two elements
-  proof : ∀ p : Person, p ≠ b → (shaves b p ↔ ¬ shaves p p)
+structure IsBarber' {t : Town} (b : Resident t) where
+  proof : ∀ p, p ≠ b → (b.shaves p ↔ ¬ p.shaves p)
 
 
-theorem solution : ∃ b, Nonempty (IsBarber' b) := by
+theorem solution : ∃ t, ∃ b : Resident t, IsBarber' b := by
   -- Use `use` to specify `b`.
   let b : Person := { name := "Oleg" }
-  use b
-  constructor
-  exact {
-    shaves p₁ p₂ := (p₁ = b) ∧ (p₂ ≠ b)
-    proof := by
-      intro p pNeqB
-      constructor
-      . intro
-        intro ⟨hPEqB, hPNeqB⟩
-        contradiction
-      . intro
-        constructor
-        . trivial
-        . exact pNeqB
+  let t : Town := {
+    people := { b }
+    shaves _ _ _ _ := False
   }
+  use t
+  let b' := Resident.mk t b (by exact Finset.mem_singleton.mpr rfl)
+  use b'
+  -- Here we need to show that `b` is a barber.
+  constructor
+  -- `constructor` turns the goal into creating the proof in the definition of
+  -- `IsBarber`.
+  intro p h_p_neq_b
+  suffices p = b' by contradiction
+  have : p.val ∈ t.people := by exact p.property
+  -- Found with "loogle"
+  apply Finset.mem_singleton.mp
+  -- Found with `exact?`
+  exact Finset.insert_eq_self.mp rfl
+
+
+-- Good job!
+-- Now let's learn about inductive types.
+
+
+-- We are actually going to use a namespace, because we are defining names that
+-- already exist in Mathlib. Defining a namespace let's you avoid this naming
+-- conflict.
+namespace SomeInductiveTypes
+
+
+inductive Tree (α : Type)
+  | leaf : Tree α
+  | branch (val : α) (left : Tree α) (right : Tree α) : Tree α
+
+
+variable {α : Type}
+
+
+def Tree.sum (t : Tree Nat) :=
+  match t with
+  | .leaf => 0
+  | .branch val left right => val + left.sum + right.sum
+
+
+def Tree.toList (t : Tree Nat) :=
+  match t with
+  | .leaf => []
+  | .branch val right left => [val] ++ left.toList ++ right.toList
+
+
+lemma sum_eq_toList_sum (t : Tree Nat) : t.sum = t.toList.sum := by
+  induction t
+  case leaf =>
+    unfold Tree.sum Tree.toList
+    -- Found with `exact?`. Could have also used `simp`
+    exact rfl
+  case branch val left right ih₁ ih₂ =>
+    unfold Tree.sum Tree.toList
+    simp
+    omega
+
+
+abbrev Var := String
+abbrev Vars := Finset String
+abbrev Assignment (vars : Vars) := (v : Var) → v ∈ vars → Bool
+
+
+def Assignment.convert {v₁ v₂} (h : v₂ ⊆ v₁ := by simp) (a : Assignment v₁) : Assignment v₂ :=
+  fun v h_v_mem_v₂ => a v (by
+    apply Finset.mem_of_subset h
+    exact h_v_mem_v₂
+  )
+
+
+inductive Formula : Vars → Type
+  | var (v : Var) : Formula { v }
+  | and {v₁ v₂} (left : Formula v₁) (right : Formula v₂) : Formula (v₁ ∪ v₂)
+  | or {v₁ v₂} (left : Formula v₁) (right : Formula v₂) : Formula (v₁ ∪ v₂)
+  | not {v₁} : Formula v₁ → Formula v₁
+  | extend {v₁ v₂} : Formula v₁ → Formula (v₁ ∪ v₂)
+
+
+def Formula.eval {vars} (f : Formula vars) (a : Assignment vars) : Bool :=
+  -- Define this function, so the lemmas below are true. Then prove them.
+  match f with
+  | var v => a v (by exact Finset.mem_singleton.mpr rfl /- `exact?` -/)
+  | or left right =>
+    left.eval a.convert ∨ right.eval a.convert
+  | and left right =>
+    left.eval a.convert ∧ right.eval a.convert
+  | not inner => ¬ inner.eval a
+  | extend inner => inner.eval a.convert
+
+
+lemma var_or_not_var_eval_eq_true {v a}
+  : ((Formula.var v).or (Formula.var v).not).eval a = true := by
+    -- Giving `simp` the definition of `eval`, it manages to simplify it
+    -- completely.
+    simp [Formula.eval]
+
+
+lemma or_not_eval_eq_true {vars} {f : Formula vars} {a}
+  : (f.or f.not).eval a = true := by
+    -- Giving `simp` the definition of `eval`, it manages to simplify it
+    -- completely.
+    -- `simp [Formula.eval, Assignment.convert]`
+    -- But here is more brutal solution:
+    unfold Formula.eval
+    simp
+    by_cases f.eval a.convert
+    case pos h =>
+      left
+      assumption
+    case neg h_not =>
+      replace h_not : f.eval a.convert = false := by
+        -- `exact?`
+        exact eq_false_of_ne_true h_not
+      right
+      unfold Formula.eval
+      simp
+      assumption
+
+
+lemma and_iff {x y h_x h_y a}
+: ((Formula.var x).and (Formula.var y)).eval a ↔ (a x h_x ∧ a y h_y) := by
+  -- Here again, the proof can be super simple...
+  simp [Formula.eval, Assignment.convert]
+
+
+class Tauto {vars} (f : Formula vars) : Prop where
+  isTrue : ∀ a, f.eval a = true
+
+
+instance {vars} {f : Formula vars} : Tauto (f.or f.not) where
+  isTrue := by
+    intro a
+    exact or_not_eval_eq_true
+
+
+instance {v₁ v₂} {f₁ : Formula v₁} {f₂ : Formula v₂} [Tauto f₁]
+: Tauto (f₁.or f₂) where
+  isTrue := by
+    intro a
+    unfold Formula.eval
+    simp
+    rw [Tauto.isTrue]
+    left
+    rfl
+
+
+-- The magic of type classes is that they can be generated by Lean when
+-- needed!
+example {v vars} {f₁ : Formula vars} {f₂ : Formula vars} {a}
+: ((((Formula.var v).or (Formula.var v).not).or f₁).or f₂).eval a = true := by
+  -- Lean automatically figures out that the formula above is `Tauto`
+  apply Tauto.isTrue
+
+
+-- Lean uses these type classes for operator overloading.
+
+-- +
+instance {v₁ v₂} : HAdd (Formula v₁) (Formula v₂) (Formula (v₁ ∪ v₂)) where
+  hAdd a b := a.or b
+-- *
+instance {v₁ v₂} : HMul (Formula v₁) (Formula v₂) (Formula (v₁ ∪ v₂)) where
+  hMul a b := a.and b
+-- unary -
+instance {vars} : Neg (Formula vars) where
+  neg := Formula.not
+
+-- Using `"x".var` instead of `Formula.var "x"`
+abbrev _root_.String.var := Formula.var
+
+-- Now we can use some arguably nicer syntax!
+def myFormula := "x".var + -"y".var
+#eval myFormula
